add value flag to untyped8, tagged, taggednumbered

src/Tagged.v
@@ -15,37 +15,37 @@ Definition function_name := nat.
 Definition rec_info := list bool.
 
 Inductive expr :=
-| Arg : expr
-| UpVar : nat -> expr
-| Call : expr -> expr -> expr
-| Constr (tag : nat) (args : list expr)
+| Value (v : value)
+| Arg
+| UpVar (idx : nat)
+| Call (f : expr) (a : expr)
+| MkConstr (tag : nat) (args : list expr)
 | Elim (cases : list (expr * rec_info)) (target : expr)
-| Close (f : function_name) (free : list expr)
+| MkClose (f : function_name) (free : list expr)
 .
+
+Inductive is_value : expr -> Prop :=
+| IsValue : forall v, is_value (Value v).
 
 Definition env := list expr.
 
-Inductive value : expr -> Prop :=
-| VConstr : forall tag args, Forall value args -> value (Constr tag args)
-| VClose : forall f free, Forall value free -> value (Close f free).
-
 Fixpoint unroll_elim (case : expr)
-                     (args : list expr)
+                     (args : list value)
                      (rec : rec_info)
                      (mk_rec : expr -> expr) : option expr :=
     match args, rec with
     | [], [] => Some case
     | arg :: args, r :: rec =>
-            let case := Call case arg in
-            let case := if r then Call case (mk_rec arg) else case in
+            let case := Call case (Value arg) in
+            let case := if r then Call case (mk_rec (Value arg)) else case in
             unroll_elim case args rec mk_rec
     | _, _ => None
     end.
 
 
 Inductive state :=
-| Run (e : expr) (l : list expr) (k : expr -> state)
-| Stop (e : expr).
+| Run (e : expr) (l : list value) (k : value -> state)
+| Stop (v : value).
 
 Inductive sstep (E : env) : state -> state -> Prop :=
 | SArg : forall l k v,
@@ -56,48 +56,45 @@ Inductive sstep (E : env) : state -> state -> Prop :=
         sstep E (Run (UpVar n) l k) (k v)
 
 | SCloseStep : forall tag vs e es l k,
-        Forall value vs ->
-        ~ value e ->
-        sstep E (Run (Close tag (vs ++ [e] ++ es)) l k)
-                (Run e l (fun v => Run (Close tag (vs ++ [v] ++ es)) l k))
+        Forall is_value vs ->
+        ~ is_value e ->
+        sstep E (Run (MkClose tag (vs ++ [e] ++ es)) l k)
+                (Run e l (fun v => Run (MkClose tag (vs ++ [Value v] ++ es)) l k))
 | SCloseDone : forall tag vs l k,
-        Forall value vs ->
-        sstep E (Run (Close tag vs) l k) (k (Close tag vs))
+        let es := map Value vs in
+        sstep E (Run (MkClose tag es) l k) (k (Close tag vs))
 
 | SConstrStep : forall fname vs e es l k,
-        Forall value vs ->
-        ~ value e ->
-        sstep E (Run (Constr fname (vs ++ [e] ++ es)) l k)
-                (Run e l (fun v => Run (Constr fname (vs ++ [v] ++ es)) l k))
+        Forall is_value vs ->
+        ~ is_value e ->
+        sstep E (Run (MkConstr fname (vs ++ [e] ++ es)) l k)
+                (Run e l (fun v => Run (MkConstr fname (vs ++ [Value v] ++ es)) l k))
 | SConstrDone : forall fname vs l k,
-        Forall value vs ->
-        sstep E (Run (Constr fname vs) l k) (k (Constr fname vs))
+        let es := map Value vs in
+        sstep E (Run (MkConstr fname es) l k) (k (Constr fname vs))
 
 | SCallL : forall e1 e2 l k,
-        ~ value e1 ->
+        ~ is_value e1 ->
         sstep E (Run (Call e1 e2) l k)
-                (Run e1 l (fun v => Run (Call v e2) l k))
+                (Run e1 l (fun v => Run (Call (Value v) e2) l k))
 | SCallR : forall e1 e2 l k,
-        value e1 ->
-        ~ value e2 ->
+        is_value e1 ->
+        ~ is_value e2 ->
         sstep E (Run (Call e1 e2) l k)
-                (Run e2 l (fun v => Run (Call e1 v) l k))
+                (Run e2 l (fun v => Run (Call e1 (Value v)) l k))
 | SMakeCall : forall fname free arg l k body,
-        Forall value free ->
-        value arg ->
         nth_error E fname = Some body ->
-        sstep E (Run (Call (Close fname free) arg) l k)
+        sstep E (Run (Call (Value (Close fname free)) (Value arg)) l k)
                 (Run body (arg :: free) k)
 
 | SElimStep : forall cases target l k,
-        ~ value target ->
+        ~ is_value target ->
         sstep E (Run (Elim cases target) l k)
-                (Run target l (fun v => Run (Elim cases v) l k))
+                (Run target l (fun v => Run (Elim cases (Value v)) l k))
 | SEliminate : forall cases tag args l k case rec e',
-        Forall value args ->
         nth_error cases tag = Some (case, rec) ->
         unroll_elim case args rec (fun x => Elim cases x) = Some e' ->
-        sstep E (Run (Elim cases (Constr tag args)) l k)
+        sstep E (Run (Elim cases (Value (Constr tag args))) l k)
                 (Run e' l k)
 .
 
@@ -122,12 +119,13 @@ Definition expr_rect_mut
         (Pl : list expr -> Type)
         (Pp : expr * rec_info -> Type)
         (Plp : list (expr * rec_info) -> Type)
+    (HValue :   forall v, P (Value v))
     (HArg :     P Arg)
     (HUpVar :   forall n, P (UpVar n))
     (HCall :    forall f a, P f -> P a -> P (Call f a))
-    (HConstr :  forall tag args, Pl args -> P (Constr tag args))
+    (HConstr :  forall tag args, Pl args -> P (MkConstr tag args))
     (HElim :    forall cases target, Plp cases -> P target -> P (Elim cases target))
-    (HClose :   forall f free, Pl free -> P (Close f free))
+    (HClose :   forall f free, Pl free -> P (MkClose f free))
     (Hnil :     Pl [])
     (Hcons :    forall e es, P e -> Pl es -> Pl (e :: es))
     (Hpair :    forall e r, P e -> Pp (e, r))
@@ -149,64 +147,44 @@ Definition expr_rect_mut
             | p :: ps => Hcons_p p ps (go_pair p) (go_pair_list ps)
             end in
         match e as e_ return P e_ with
+        | Value v => HValue v
         | Arg => HArg
         | UpVar n => HUpVar n
         | Call f a => HCall f a (go f) (go a)
-        | Constr tag args => HConstr tag args (go_list args)
+        | MkConstr tag args => HConstr tag args (go_list args)
         | Elim cases target => HElim cases target (go_pair_list cases) (go target)
-        | Close f free => HClose f free (go_list free)
+        | MkClose f free => HClose f free (go_list free)
         end in go e.
 
 (* Useful wrapper for `expr_rect_mut with (Pl := Forall P)` *)
 Definition expr_ind' (P : expr -> Prop) (Pp : (expr * rec_info) -> Prop)
+    (HValue :   forall v, P (Value v))
     (HArg :     P Arg)
     (HUpVar :   forall n, P (UpVar n))
     (HCall :    forall f a, P f -> P a -> P (Call f a))
-    (HConstr :  forall c args, Forall P args -> P (Constr c args))
+    (HConstr :  forall c args, Forall P args -> P (MkConstr c args))
     (HElim :    forall cases target, Forall Pp cases -> P target -> P (Elim cases target))
-    (HClose :   forall f free, Forall P free -> P (Close f free))
+    (HClose :   forall f free, Forall P free -> P (MkClose f free))
     (Hpair :    forall e r, P e -> Pp (e, r))
     (e : expr) : P e :=
     ltac:(refine (@expr_rect_mut P (Forall P) Pp (Forall Pp)
-        HArg HUpVar HCall HConstr HElim HClose _ _ Hpair _ _ e); eauto).
+        HValue HArg HUpVar HCall HConstr HElim HClose _ _ Hpair _ _ e); eauto).
 
 (* Useful wrapper for `expr_rect_mut with (Pl := Forall P)` *)
 Definition expr_ind'' (P : expr -> Prop)
+    (HValue :   forall v, P (Value v))
     (HArg :     P Arg)
     (HUpVar :   forall n, P (UpVar n))
     (HCall :    forall f a, P f -> P a -> P (Call f a))
-    (HConstr :  forall c args, Forall P args -> P (Constr c args))
+    (HConstr :  forall c args, Forall P args -> P (MkConstr c args))
     (HElim :    forall cases target,
         Forall (fun c => P (fst c)) cases ->
         P target ->
         P (Elim cases target))
-    (HClose :   forall f free, Forall P free -> P (Close f free))
+    (HClose :   forall f free, Forall P free -> P (MkClose f free))
     (e : expr) : P e :=
     ltac:(refine (@expr_rect_mut P (Forall P) (fun c => P (fst c)) (Forall (fun c => P (fst c)))
-        HArg HUpVar HCall HConstr HElim HClose _ _ _ _ _ e); eauto).
-
-
-(*
- * value_ok
- *)
-
-
-Inductive value_ok (E : env) : expr -> Prop :=
-| ConstrOk :
-        forall tag args,
-        Forall (value_ok E) args ->
-        value_ok E (Constr tag args)
-| CloseOk : forall f free body,
-        nth_error E f = Some body ->
-        Forall (value_ok E) free ->
-        value_ok E (Close f free).
-
-Theorem value_ok_value : forall E e, value_ok E e -> value e.
-induction e using expr_ind''; intro Hok; invc Hok.
-- constructor. list_magic_on (args, tt).
-- constructor. list_magic_on (free, tt).
-Qed.
-Hint Resolve value_ok_value.
+        HValue HArg HUpVar HCall HConstr HElim HClose _ _ _ _ _ e); eauto).
 
 
 (*
@@ -237,35 +215,21 @@ Require Semantics.
 Definition prog_type : Type := list expr * list metadata.
 Definition valtype := HigherValue.value.
 
-Inductive expr_value : expr -> valtype -> Prop :=
-| EvConstr : forall tag args1 args2,
-        Forall2 expr_value args1 args2 ->
-        expr_value (Constr tag args1)
-                   (HigherValue.Constr tag args2)
-| EvClose : forall tag free1 free2,
-        Forall2 expr_value free1 free2 ->
-        expr_value (Close tag free1)
-                   (HigherValue.Close tag free2)
-.
-
 Definition initial_env (prog : prog_type) : env := fst prog.
 
 Inductive is_callstate (prog : prog_type) : valtype -> valtype -> state -> Prop :=
-| IsCallstate : forall fname free free_e av ae body,
+| IsCallstate : forall fname free av body,
         nth_error (fst prog) fname = Some body ->
-        let fv := HigherValue.Close fname free in
-        expr_value ae av ->
-        Forall2 expr_value free_e free ->
+        let fv := Close fname free in
         HigherValue.public_value (snd prog) fv ->
         HigherValue.public_value (snd prog) av ->
         is_callstate prog fv av
-            (Run body (ae :: free_e) Stop).
+            (Run body (av :: free) Stop).
 
 Inductive final_state (prog : prog_type) : state -> valtype -> Prop :=
-| FinalState : forall e v,
-        expr_value e v ->
+| FinalState : forall v,
         HigherValue.public_value (snd prog) v ->
-        final_state prog (Stop e) v.
+        final_state prog (Stop v) v.
 
 Definition semantics (prog : prog_type) : Semantics.semantics :=
   @Semantics.Semantics_gen state env valtype
@@ -273,31 +237,3 @@ Definition semantics (prog : prog_type) : Semantics.semantics :=
                  (sstep)
                  (final_state prog)
                  (initial_env prog).
-
-
-Lemma expr_value_value : forall e v,
-    expr_value e v ->
-    value e.
-induction e using expr_rect_mut with
-    (Pl := fun es => forall vs,
-        Forall2 expr_value es vs ->
-        Forall value es)
-    (Pp := fun e => forall v,
-        expr_value (fst e) v ->
-        value (fst e))
-    (Plp := fun es => forall vs,
-        Forall2 (fun e v => expr_value (fst e) v) es vs ->
-        Forall (fun e => value (fst e)) es) ;
-intros0 Hev; try solve [invc Hev + simpl in *; eauto].
-
-- invc Hev. constructor. eauto.
-- invc Hev. constructor. eauto.
-Qed.
-Hint Resolve expr_value_value.
-
-Lemma expr_value_value_list : forall e v,
-    Forall2 expr_value e v ->
-    Forall value e.
-induction e; intros0 Hev; invc Hev; eauto using expr_value_value.
-Qed.
-Hint Resolve expr_value_value_list.
