src/Untyped8.v
@@ -7,42 +7,37 @@ Require Import HighestValues.
 
 
 Inductive expr :=
+| Value (v : value)
 | Arg
 | UpVar (idx : nat)
 | App (f : expr) (a : expr)
-| Constr (ctor : constr_name) (args : list expr)
-| Close (fname : nat) (free : list expr)
+| MkConstr (ctor : constr_name) (args : list expr)
+| MkClose (fname : nat) (free : list expr)
 | Elim (ty : type_name) (cases : list expr) (target : expr)
 .
 
 Inductive is_value : expr -> Prop :=
-| IsVConstr : forall ctor args,
-        Forall is_value args ->
-        is_value (Constr ctor args)
-| IsVClose : forall fname free,
-        Forall is_value free ->
-        is_value (Close fname free)
-.
+| IsValue : forall v, is_value (Value v).
 
 
 Inductive state :=
-| Run (e : expr) (l : list expr) (k : expr -> state)
-| Stop (v : expr)
+| Run (e : expr) (l : list value) (k : value -> state)
+| Stop (v : value)
 .
 
 
 (* helper function for proceeding into an elim *)
 Fixpoint unroll_elim' (case : expr)
                       (ctor : constr_name)
-                      (args : list expr)
+                      (args : list value)
                       (mk_rec : expr -> expr)
                       (idx : nat) : expr :=
     match args with
     | [] => case
     | arg :: args =>
-            let case := App case arg in
+            let case := App case (Value arg) in
             let case := if ctor_arg_is_recursive ctor idx
-                then App case (mk_rec arg) else case in
+                then App case (mk_rec (Value arg)) else case in
             unroll_elim' case ctor args mk_rec (S idx)
     end.
 
@@ -51,12 +46,12 @@ Definition unroll_elim case ctor args mk_rec :=
 
 (* the actual step relation *)
 Inductive sstep (g : list expr) : state -> state -> Prop :=
-| SArg : forall (l : list expr) k v,
+| SArg : forall (l : list value) k v,
         nth_error l 0 = Some v ->
         sstep g (Run (Arg) l k)
                 (k v)
 
-| SUpVar : forall idx (l : list expr) k v,
+| SUpVar : forall idx (l : list value) k v,
         nth_error l (S idx) = Some v ->
         sstep g (Run (UpVar idx) l k)
                 (k v)
@@ -64,21 +59,18 @@ Inductive sstep (g : list expr) : state -> state -> Prop :=
 | SAppL : forall (e1 : expr) (e2 : expr) l k,
         ~ is_value e1 ->
         sstep g (Run (App e1 e2) l k)
-                (Run e1 l (fun v => Run (App v e2) l k))
+                (Run e1 l (fun v => Run (App (Value v) e2) l k))
 
 | SAppR : forall (e1 : expr) (e2 : expr) l k,
         is_value e1 ->
         ~ is_value e2 ->
         sstep g (Run (App e1 e2) l k)
-                (Run e2 l (fun v => Run (App e1 v) l k))
+                (Run e2 l (fun v => Run (App e1 (Value v)) l k))
 
 | SMakeCall : forall fname free arg l k body,
-        Forall is_value free ->
-        is_value arg ->
         nth_error g fname = Some body ->
-        sstep g (Run (App (Close fname free) arg) l k)
+        sstep g (Run (App (Value (Close fname free)) (Value arg)) l k)
                 (Run body (arg :: free) k)
-
 | SConstrStep : forall
             (ctor : constr_name)
             (vs : list expr)
@@ -87,15 +79,15 @@ Inductive sstep (g : list expr) : state -> state -> Prop :=
             l k,
         Forall is_value vs ->
         ~ is_value e ->
-        sstep g (Run (Constr ctor (vs ++ e :: es)) l k)
-                (Run e l (fun v => Run (Constr ctor (vs ++ v :: es)) l k))
+        sstep g (Run (MkConstr ctor (vs ++ e :: es)) l k)
+                (Run e l (fun v => Run (MkConstr ctor (vs ++ (Value v) :: es)) l k))
 
 | SConstrDone : forall
             (ctor : constr_name)
-            (vs : list expr)
+            (vs : list value)
             l k,
-        Forall is_value vs ->
-        sstep g (Run (Constr ctor vs) l k)
+        let es := map Value vs in
+        sstep g (Run (MkConstr ctor es) l k)
                 (k (Constr ctor vs))
 
 | SCloseStep : forall
@@ -106,15 +98,15 @@ Inductive sstep (g : list expr) : state -> state -> Prop :=
             l k,
         Forall is_value vs ->
         ~ is_value e ->
-        sstep g (Run (Close fname (vs ++ e :: es)) l k)
-                (Run e l (fun v => Run (Close fname (vs ++ v :: es)) l k))
+        sstep g (Run (MkClose fname (vs ++ e :: es)) l k)
+                (Run e l (fun v => Run (MkClose fname (vs ++ (Value v) :: es)) l k))
 
 | SCloseDone : forall
             (fname : nat)
-            (vs : list expr)
+            (vs : list value)
             l k,
-        Forall is_value vs ->
-        sstep g (Run (Close fname vs) l k)
+        let es := map Value vs in
+        sstep g (Run (MkClose fname es) l k)
                 (k (Close fname vs))
 
 | SElimTarget : forall
@@ -124,22 +116,21 @@ Inductive sstep (g : list expr) : state -> state -> Prop :=
             l k,
         ~ is_value target ->
         sstep g (Run (Elim ty cases target) l k)
-                (Run target l (fun v => Run (Elim ty cases v) l k))
+                (Run target l (fun v => Run (Elim ty cases (Value v)) l k))
 
 | SEliminate : forall
             (ty : type_name)
             (cases : list expr)
             (ctor : constr_name)
-            (args : list expr)
+            (args : list value)
             (case : expr)
             (result : expr)
             l k,
-        Forall is_value args ->
         is_ctor_for_type ty ctor ->
         constructor_arg_n ctor = length args ->
         nth_error cases (constructor_index ctor) = Some case ->
         unroll_elim case ctor args (Elim ty cases) = result ->
-        sstep g (Run (Elim ty cases (Constr ctor args)) l k)
+        sstep g (Run (Elim ty cases (Value (Constr ctor args))) l k)
                 (Run result l k)
 .
 
@@ -150,11 +141,12 @@ Inductive sstep (g : list expr) : state -> state -> Prop :=
  *)
 
 Definition expr_rect_mut (P : expr -> Type) (Pl : list expr -> Type)
+    (HValue :   forall v, P (Value v))
     (HArg :     P Arg)
     (HUpVar :   forall n, P (UpVar n))
     (HApp :     forall f a, P f -> P a -> P (App f a))
-    (HConstr :  forall ctor args, Pl args -> P (Constr ctor args))
-    (HClose :   forall fname free, Pl free -> P (Close fname free))
+    (HConstr :  forall ctor args, Pl args -> P (MkConstr ctor args))
+    (HClose :   forall fname free, Pl free -> P (MkClose fname free))
     (HElim :    forall ty cases target, Pl cases -> P target -> P (Elim ty cases target))
     (Hnil :     Pl [])
     (Hcons :    forall e es, P e -> Pl es -> Pl (e :: es))
@@ -166,67 +158,26 @@ Definition expr_rect_mut (P : expr -> Type) (Pl : list expr -> Type)
             | e :: es => Hcons e es (go e) (go_list es)
             end in
         match e as e_ return P e_ with
+        | Value v => HValue v
         | Arg => HArg
         | UpVar n => HUpVar n
         | App f a => HApp f a (go f) (go a)
-        | Constr ctor args => HConstr ctor args (go_list args)
-        | Close fname free => HClose fname free (go_list free)
+        | MkConstr ctor args => HConstr ctor args (go_list args)
+        | MkClose fname free => HClose fname free (go_list free)
         | Elim ty cases target => HElim ty cases target (go_list cases) (go target)
         end in go e.
 
 Definition expr_rect_mut' (P : expr -> Type) (Pl : list expr -> Type)
-    HArg HUpVar HApp HConstr HClose HElim Hnil Hcons
+    HValue HArg HUpVar HApp HConstr HClose HElim Hnil Hcons
     : (forall e, P e) * (forall es, Pl es) :=
     let go := expr_rect_mut P Pl 
-        HArg HUpVar HApp HConstr HClose HElim Hnil Hcons
+        HValue HArg HUpVar HApp HConstr HClose HElim Hnil Hcons
         in
     let fix go_list es :=
         match es as es_ return Pl es_ with
         | [] => Hnil
         | e :: es => Hcons e es (go e) (go_list es)
         end in (go, go_list).
-
-
-
-
-Inductive expr_value : expr -> value -> Prop :=
-| EvConstr : forall ctor args_e args_v,
-        Forall2 expr_value args_e args_v ->
-        expr_value (Constr ctor args_e) (HighestValues.Constr ctor args_v)
-| EvClose : forall fname free_e free_v,
-        Forall2 expr_value free_e free_v ->
-        expr_value (Close fname free_e) (HighestValues.Close fname free_v)
-.
-
-
-Lemma expr_value_is_value : forall e v,
-    expr_value e v ->
-    is_value e.
-mut_induction e using expr_rect_mut' with
-    (Pl := fun es => forall vs,
-        Forall2 expr_value es vs ->
-        Forall is_value es);
-[ intros0 Hev; invc Hev; try solve [econstructor; eauto].. | ].
-
-- finish_mut_induction expr_value_is_value using list.
-Qed exporting.
-
-
-Lemma is_value_expr_value : forall e,
-    is_value e ->
-    exists v, expr_value e v.
-mut_induction e using expr_rect_mut' with
-    (Pl := fun es =>
-        Forall is_value es ->
-        exists vs, Forall2 expr_value es vs);
-[ intros0 Hval; invc Hval; try solve [econstructor; eauto].. | ].
-
-- destruct (IHe **). eexists. econstructor. eauto.
-- destruct (IHe **). eexists. econstructor. eauto.
-- destruct (IHe **), (IHe0 **). eexists. econstructor; eauto.
-
-- finish_mut_induction is_value_expr_value using list.
-Qed exporting.
 
 
 
@@ -239,19 +190,16 @@ Definition valtype := value.
 Definition initial_env (prog : prog_type) : env := fst prog.
 
 Inductive is_callstate (prog : prog_type) : valtype -> valtype -> state -> Prop :=
-| IsCallstate : forall fname free av free_e ae body,
+| IsCallstate : forall fname free av body,
         nth_error (fst prog) fname = Some body ->
         let fv := HighestValues.Close fname free in
-        Forall2 expr_value free_e free ->
-        expr_value ae av ->
         is_callstate prog fv av
-            (Run body (ae :: free_e) Stop).
+            (Run body (av :: free) Stop).
 
 Inductive final_state (prog : prog_type) : state -> valtype -> Prop :=
-| FinalState : forall e v,
-        expr_value e v ->
+| FinalState : forall v,
         HighestValues.public_value (snd prog) v ->
-        final_state prog (Stop e) v.
+        final_state prog (Stop v) v.
 
 Definition semantics (prog : prog_type) : Semantics.semantics :=
   @Semantics_gen state env valtype
